PiLL/PiLL/Framework/Substitution.lean
@@ -569,6 +569,129 @@ theorem Typing.subst_name (𝒢 : HyperEnv) (P : Proc) (𝒟 : ⊢ P ∷ 𝒢) (
         apply ih ⟨⟨hFresh.1, ⟨hFresh.2.1, hSafe.2.1⟩⟩, ⟨hFresh.2.2, hSafe.1⟩⟩ hSafe.2.2
 
 
+lemma Types.subst_eq_self {T A : Types} {X : TVar} {hft : X ∉ T.freeTypes} :
+  T.subst A X = T := by
+  induction T <;> simp_all [Types.subst, Types.freeTypes, ← ne_eq]
+
+  case var | varDual=>
+    intro h
+    subst h
+    contradiction
+
+  case forall_ ih | exist_ ih =>
+    split_ifs with h
+    · subst h ; rfl
+    · simp_all only [forall_.injEq, exist_.injEq, true_and, ← ne_eq]
+      apply ih
+      intro h_contra
+      simp [h_contra] at hft
+      subst hft
+      contradiction
+
+lemma Types.freeTypes_dual_eq (T : Types) : T.dual.freeTypes = T.freeTypes := by
+  induction T <;> simp_all [Types.freeTypes, Types.dual]
+
+@[simp] lemma Types.not_mem_ft_subst {T A : Types} {X Y : TVar}
+  (hT : Y ∉ T.freeTypes) (hA : Y ∉ A.freeTypes) (hneq : Y ≠ X) :
+  Y ∉ (T.subst A X).freeTypes := by
+  induction T <;> simp_all [Types.subst, Types.freeTypes, ← ne_eq]
+
+  case var =>
+    split_ifs with h
+    · exact hA
+    · simp [Types.freeTypes] ; exact hT
+
+  case varDual =>
+    split_ifs with h
+    · simp [Types.freeTypes_dual_eq] ; exact hA
+    · simp [Types.freeTypes] ; exact hT
+
+  case forall_ A' ih | exist_ A' ih =>
+    split_ifs with h1
+    · simp [Types.freeTypes]
+      intro hin
+      have heq : Y = X := by
+        rw [← h1]
+        apply hT hin
+      contradiction
+    · simp only [Types.freeTypes, Finset.mem_sdiff, Finset.mem_singleton]
+      intro h2
+      have hog : Y ∈ A'.freeTypes := by
+        by_contra hc
+        apply ih at hc
+        exact hc h2.1
+      apply hT at hog
+      exact h2.2 hog
+
+lemma Types.subst_subst (T A B : Types) (X : TVar) :
+  (T.subst A X).subst B X = T.subst (A.subst B X) X := by
+  induction T generalizing A B <;> simp_all [Types.subst]
+
+  case var | varDual =>
+    split_ifs with h
+    · (try erw [← Types.subst_dual]) ; rfl
+    · simp [Types.subst]
+      intro a
+      contradiction
+
+  case forall_ ih | exist_ ih =>
+    split_ifs with h
+    · simp [Types.subst]
+    · simp [Types.subst]
+      simp [h]
+      apply ih
+
+@[simp] lemma Types.subst_eq_self_of_not_mem (T A : Types) (X : TVar)
+  (h : X ∉ T.freeTypes) : T.subst A X = T := by
+  induction T <;> simp_all [Types.subst, Types.freeTypes]
+  case var | varDual =>
+    intro h
+    subst h
+    contradiction
+
+  case forall_ ih | exist_ ih =>
+    split_ifs with h1
+    · subst h1 ; rfl
+    · congr
+      apply ih
+      intro hin
+      apply h at hin
+      rw [hin] at h1
+      contradiction
+
+lemma Types.subst_commute (T A B : Types) (X Y : TVar) (hne : Y ≠ X) (hft : Y ∉ A.freeTypes) :
+  (T.subst B Y).subst A X = (T.subst A X).subst (B.subst A X) Y := by
+  induction T generalizing A B X Y <;> simp_all [Types.subst]
+
+  case var =>
+    split_ifs with h1 h2 h3 <;> simp_all [Types.subst]
+
+  case varDual =>
+    split_ifs with h1 h2 h3
+    · simp_all
+    · simp_all [Types.subst]
+      erw [← Types.subst_dual]
+      rfl
+    · simp_all [Types.subst]
+      symm
+      apply Types.subst_eq_self_of_not_mem
+      simp [Types.freeTypes_dual_eq, hft]
+    · simp_all [Types.subst]
+
+  case forall_ ih =>
+    split_ifs with h1 h2 h3 <;> simp_all [Types.subst]
+    sorry -- FIXME: Currently assuming Barendregt (add frehsness contraint?)
+
+  case exist_ =>
+    split_ifs with h1 h2 h3 <;> try simp_all [Types.subst]
+    sorry -- FIXME: Currently assuming Barendregt (add frehsness contraint?)
+
+
+
+
+
+
+
 @[simp] lemma Proc.substTypes_nil {A : Types} {X : TVar} : 𝟘{A // X} = 𝟘 := by rfl
 
 @[simp] lemma Proc.substTypes_link {x y : PName} {A : Types} {X : TVar} :
@@ -586,8 +709,15 @@ theorem Typing.subst_name (𝒢 : HyperEnv) (P : Proc) (𝒟 : ⊢ P ∷ 𝒢) (
 @[simp] lemma Proc.substTypes_output {x : PName} {P : Proc} {T A : Types} {X : TVar} :
   (x⟦T⟧․P){A // X} = x⟦T{A // X}⟧․(P{A // X}) := by rfl
 
--- @[simp] lemma Proc.substTypes_forall {x : PName} {P : Proc} {A : Types} {X : TVar} :
---   (x⸨X⸩․P){A // X} = /- some expression -/ := by sorry
+
+@[simp] lemma Proc.substTypes_input_match {x : PName} {P : Proc} {A : Types} {X : TVar} :
+  (x⸨X⸩․P){A // X} = x⸨X⸩․P := by
+  simp [HasSubst.subst, Proc.substTypes, HasParen.paren]
+
+@[simp] lemma Proc.substTypes_input_diff {x : PName} {P : Proc} {A : Types} {X Y : TVar}
+  (hneq : Y ≠ X) : (x⸨Y⸩․P){A // X} = x⸨Y⸩․P{A // X} := by
+  simp_all [HasSubst.subst, Proc.substTypes, HasParen.paren]
+
 
 
 
@@ -604,7 +734,7 @@ theorem Typing.subst_name (𝒢 : HyperEnv) (P : Proc) (𝒟 : ⊢ P ∷ 𝒢) (
   simp only [HasSubst.subst, Env.substTypes, Env.merge, Finset.image_union]
 
 @[simp]
-lemma Env.names_substTypes (Γ : Env) (A : Types) (X : TVar) :
+lemma Env.names_substTypes {Γ : Env} {A : Types} {X : TVar} :
   (Γ{A // X}).names = Γ.names := by
   simp only [Env.names, Env.substTypes, HasSubst.subst, Finset.image_image]
   apply Finset.image_congr
@@ -614,6 +744,54 @@ lemma Env.names_substTypes (Γ : Env) (A : Types) (X : TVar) :
 @[simp] lemma Env.substTypes_preserves_disjoint {Γ Δ : Env} {A : Types} {X : TVar} :
   Γ{A // X}.disjoint Δ{A // X} = Γ.disjoint Δ := by
   simp only [Env.disjoint, Env.names_substTypes]
+
+@[simp] lemma Env.substTypes_eq_self_of_not_mem {Γ : Env} {A : Types} {X : TVar}
+  (h : X ∉ ft(Γ)ₑ) : Γ{A // X} = Γ := by
+  simp only [HasSubst.subst, Env.substTypes]
+  conv_rhs => rw [← Finset.image_id (s := Γ)]
+  apply Finset.image_congr
+  intro ⟨n, T⟩ hin
+  simp
+  apply Types.subst_eq_self
+  simp only [Env.freeTypes, Finset.mem_biUnion, not_exists, not_and] at h
+  exact h (n, T) hin
+
+@[simp] lemma Env.not_mem_ft_substTypes {Γ : Env} {A : Types} {X Y : TVar} {hΓ : Y ∉ ft(Γ)ₑ}
+  {hA : Y ∉ A.freeTypes} {hneq : Y ≠ X} : Y ∉ ft(Γ{A // X})ₑ := by
+  simp only [HasSubst.subst, Env.substTypes, Env.freeTypes, Finset.mem_biUnion,
+    not_exists, not_and]
+  intro p hp
+  rcases Finset.mem_image.mp hp with ⟨op, hom, heq⟩
+  subst heq
+  apply Types.not_mem_ft_subst
+  · rw [Env.freeTypes] at hΓ
+    simp only [Finset.mem_biUnion, not_exists, not_and] at hΓ
+    exact hΓ op hom
+  · exact hA
+  · exact hneq
+
+
+
+
+@[simp] lemma Env.substTypes_mk {x : PName} {T A : Types} {X : TVar} :
+  (x ∶ T){A // X} = x ∶ T.subst A X := by
+  simp only [HasSubst.subst, Env.substTypes, Env.mk, Finset.image_singleton]
+
+@[simp] lemma Env.freeTypes_empty :
+  ft(∅)ₑ = ∅ := by simp only [Env.freeTypes, Finset.biUnion_empty]
+
+@[simp] lemma Env.freeTypes_singleton {x : PName} {A : Types} :
+  ft((x ∶ A : Env))ₑ = A.freeTypes := by
+  simp only [Env.freeTypes, Env.freeTypes, Env.mk, Finset.singleton_biUnion]
+
+@[simp] lemma Env.freeTypes_distributes {Γ Δ : Env} :
+   (ft(Γ‚ Δ)ₑ) = (ft(Γ)ₑ ∪ ft(Δ)ₑ) := by
+   simp only [Env.merge, Env.freeTypes, Finset.biUnion_union]
+
+@[simp] lemma Env.freeTypes_notMem_merge {Γ Δ : Env} {X : TVar} :
+   (X ∉ ft(Γ‚ Δ)ₑ) = (X ∉ ft(Γ)ₑ ∧ X ∉ ft(Δ)ₑ) := by
+   simp only [Env.freeTypes_distributes, Finset.notMem_union]
+
 
 
 
@@ -632,7 +810,7 @@ lemma Env.names_substTypes (Γ : Env) (A : Types) (X : TVar) :
   simp only [HasSubst.subst, HyperEnv.substTypes, HyperEnv.merge, Finset.image_union]
 
 @[simp]
-lemma HyperEnv.names_substTypes (𝒢 : HyperEnv) (A : Types) (X : TVar) :
+lemma HyperEnv.names_substTypes {𝒢 : HyperEnv} {A : Types} {X : TVar} :
   (𝒢{A // X}).names = 𝒢.names := by
   simp only [HyperEnv.names, HyperEnv.substTypes, HasSubst.subst]
   rw [Finset.image_biUnion]
@@ -642,14 +820,23 @@ lemma HyperEnv.names_substTypes (𝒢 : HyperEnv) (A : Types) (X : TVar) :
   𝒢{A // X}.disjoint ℋ{A // X} = 𝒢.disjoint ℋ := by
   simp only [HyperEnv.disjoint, HyperEnv.names_substTypes]
 
+@[simp] lemma HyperEnv.freeTypes_empty :
+  ft(∅)ₕ = ∅ := by simp only [HyperEnv.freeTypes, Finset.biUnion_empty]
 
-@[simp]
-lemma Env.substTypes_mk (x : PName) (T A : Types) (X : TVar) :
-  (x ∶ T){A // X} = x ∶ T.subst A X := by
-  simp only [HasSubst.subst, Env.substTypes, Env.mk, Finset.image_singleton]
+@[simp] lemma HyperEnv.freeTypes_singleton {Γ : Env} :
+  ft(({Γ} : HyperEnv))ₕ = ft(Γ)ₑ := by
+  simp only [HyperEnv.freeTypes, HyperEnv.freeTypes, Finset.singleton_biUnion]
+
+@[simp] lemma HyperEnv.freeTypes_distributes {𝒢 ℋ : HyperEnv} :
+   (ft(𝒢 |ₕ ℋ)ₕ) = (ft(𝒢)ₕ ∪ ft(ℋ)ₕ) := by
+   simp only [HyperEnv.merge, HyperEnv.freeTypes, Finset.biUnion_union]
+
+@[simp] lemma HyperEnv.freeTypes_notMem_merge {𝒢 ℋ : HyperEnv} {X : TVar} :
+   (X ∉ ft(𝒢 |ₕ ℋ)ₕ) = (X ∉ ft(𝒢)ₕ ∧ X ∉ ft(ℋ)ₕ) := by
+   simp only [HyperEnv.freeTypes_distributes, Finset.notMem_union]
 
 
-
+attribute [simp] Types.freeTypes
 
 
 theorem Typing.subst_types {𝒢 : HyperEnv} {P : Proc} {𝒟 : ⊢ P ∷ 𝒢}
@@ -673,13 +860,21 @@ theorem Typing.subst_types {𝒢 : HyperEnv} {P : Proc} {𝒟 : ⊢ P ∷ 𝒢}
     apply Typing.one
     · exact ih
 
-  case bot hf _ ih | w hf _ ih=>
-    constructor
+  case bot hf _ ih =>
+    apply Typing.bot
     · simp ; exact hf
-    · exact ih
+    · apply ih
 
-  case oplus₁ ih | oplus₂ ih | quest ih =>
-    constructor
+  case oplus₁ ih =>
+    apply Typing.oplus₁
+    exact ih
+
+  case oplus₂ ih =>
+    apply Typing.oplus₂
+    exact ih
+
+  case quest ih =>
+    apply Typing.quest
     exact ih
 
   case amp ihP ihQ =>
@@ -693,6 +888,11 @@ theorem Typing.subst_types {𝒢 : HyperEnv} {P : Proc} {𝒟 : ⊢ P ∷ 𝒢}
     · simp ; exact hf
     · exact ih
 
+  case w hf _ ih =>
+    apply Typing.w
+    · simp ; exact hf
+    · apply ih
+
   case bang hsu ih =>
     all_goals
       apply Typing.bang
@@ -704,14 +904,35 @@ theorem Typing.subst_types {𝒢 : HyperEnv} {P : Proc} {𝒟 : ⊢ P ∷ 𝒢}
     simp [HasSubst.subst, Types.subst] at ⊢ ih
     split_ifs with h
     · apply Typing.exists_
-      sorry
+      simp_all only [HasSubst.subst, Types.subst_subst]
     · apply Typing.exists_
-      sorry
+      rw [Types.subst_commute] at ih
+      · exact ih
+      · exact h
+      · sorry -- FIXME: Currently assuming Barendregt (add freshness condition?)
 
-  case forall_ ft ih =>
-    simp [HasSubst.subst, Types.subst] at ⊢ ih
-    split_ifs
-    · apply Typing.forall_ -- FIXME: Missing Proc.substTypes_forall
+
+
+  case forall_ D ft ih =>
+    conv_lhs => rhs ; rhs ; simp [HasSubst.subst, Types.subst]
+    split_ifs with h
+    · subst h
+      rw [Proc.substTypes_input_match]
+      apply Typing.forall_
+      · rw [Env.substTypes_eq_self_of_not_mem]
+        · exact D
+        · exact ft
+      · rw [Env.substTypes_eq_self_of_not_mem]
+        · exact ft
+        · exact ft
+    · rw [Proc.substTypes_input_diff]
+      · apply Typing.forall_
+        · apply ih
+        · apply Env.not_mem_ft_substTypes
+          · exact ft
+          · sorry -- FIXME: Currently assuming Barendregt (could also add h : A.freeTypes = ∅)
+          · exact h
+      · exact h
 
   case tensor hf hneq hDisj _ ih =>
     apply Typing.tensor
@@ -734,4 +955,4 @@ theorem Typing.subst_types {𝒢 : HyperEnv} {P : Proc} {𝒟 : ⊢ P ∷ 𝒢}
     · rw [Env.substTypes_preserves_disjoint]
       exact hDisj
     · rw [HyperEnv.merge_assoc]
-      exact ih
+      · exact ih
